proof lemma 8.2.2

TaplLean/TypedArith/Type.lean
@@ -1,37 +1,79 @@
 import TaplLean.TypedArith.Arith
-open Term
 
 inductive Ty : Type where
   | TNat
   | TBool
+  deriving DecidableEq
 
-inductive HasTy : Term → Ty → Prop where
-  | has_ty_tru : HasTy tru TBool
-  | has_ty_fls : HasTy fls TBool
-  | has_ty_if : ∀ {t1 t2 t3 : Term} {T : Ty},
-      HasTy t1 TBool → HasTy t2 T → HasTy t3 T
-      → HasTy (ite t1 t2 t3) T
-  | has_ty_zero : HasTy zero TNat
-  | has_ty_succ : ∀ {t : Term},
-      HasTy t TNat → HasTy (succ t) TNat
-  | has_ty_pred : ∀ {t : Term},
-      HasTy t TNat → HasTy (pred t) TNat
-  | has_ty_iszero : ∀ {t : Term},
-      HasTy t TNat → HasTy (iszero t) TBool
+open Term
+open Ty
 
-notation:10 "⊢ " e " : " τ => HasTy e τ
+-- 型付け関係
+inductive WellTyped : Term → Ty → Prop where
+  | wt_tru : WellTyped tru TBool
+  | wt_fls : WellTyped fls TBool
+  | wt_if : ∀ {t1 t2 t3 : Term} {T : Ty},
+      WellTyped t1 TBool → WellTyped t2 T → WellTyped t3 T
+      → WellTyped (ite t1 t2 t3) T
+  | wt_zero : WellTyped zero TNat
+  | wt_succ : ∀ {t : Term},
+      WellTyped t TNat → WellTyped (succ t) TNat
+  | wt_pred : ∀ {t : Term},
+      WellTyped t TNat → WellTyped (pred t) TNat
+  | wt_iszero : ∀ {t : Term},
+      WellTyped t TNat → WellTyped (iszero t) TBool
 
-open HasTy
+notation:10 "⊢ " e " : " τ => WellTyped e τ
+
+open WellTyped
 
 example : ⊢ pred (succ (pred (succ zero))) : TNat := by
-  apply has_ty_pred
-  apply has_ty_succ
-  apply has_ty_pred
-  apply has_ty_succ
-  apply has_ty_zero
+  apply wt_pred
+  apply wt_succ
+  apply wt_pred
+  apply wt_succ
+  apply wt_zero
   done
 
+-- 補題8.2.2 逆転補題 START
 theorem rev_ty_tru : ∀ {T : Ty}, (⊢ tru : T) → T = TBool := by
-  intros T h
-  sorry
-  -- have ht : ⊢ tru : TBool := has_ty_tru
+  intro T h
+  cases h
+  rfl
+
+theorem rev_ty_fls : ∀ {T : Ty}, (⊢ fls : T) → T = TBool := by
+  intro T h
+  cases h
+  rfl
+
+theorem rev_ty_ite : ∀ {T : Ty} {t1 t2 t3 : Term},
+  (⊢ ite t1 t2 t3 : T) → WellTyped t1 TBool ∧ WellTyped t2 T ∧ WellTyped t3 T
+  := by
+  intro T t1 t2 t3 h
+  cases h
+  apply And.intro; assumption
+  apply And.intro <;> assumption
+
+theorem rev_ty_zero : ∀ {T : Ty}, (⊢ zero : T) → T = TNat := by
+  intro T h; cases h; rfl
+
+theorem rev_ty_succ :
+  ∀ {T : Ty} {t : Term}, (⊢ succ t : T) → T = TNat ∧ (⊢ t : TNat)
+  := by
+  intro T t h; cases h
+  apply And.intro; rfl; assumption
+
+theorem rev_ty_pred :
+  ∀ {T : Ty} {t : Term}, (⊢ pred t : T) → T = TNat ∧ (⊢ t : TNat)
+  := by
+  intro T t h; cases h
+  apply And.intro; rfl; assumption
+
+theorem rev_ty_iszero :
+  ∀ {T : Ty} {t : Term}, (⊢ iszero t : T) → T = TBool ∧ (⊢ t : TNat)
+  := by
+  intro T t h; cases h
+  apply And.intro; rfl; assumption
+-- 補題8.2.2 逆転補題 END
+
+-- 演習8.2.3 START
